Introduce n_ag

nola/examples/logic/iris.v
@@ -13,14 +13,21 @@ Variant nInvd : Type :=
 | (* non-atomic *) nInvd_na
     (p : na_inv_pool_name) (i : positive) (P : nPropS (;ᵞ)).
 
+(** Agreement *)
+Class agreeG A Σ := { agree_inG :: inG Σ (agreeR (leibnizO A)) }.
+Definition agreeΣ A : gFunctors := #[GFunctor (agreeR (leibnizO A))].
+#[export] Instance subG_agreeΣ `{!subG (agreeΣ A) Σ} : agreeG A Σ.
+Proof. solve_inG. Qed.
+
 (** [nintpGS]: Iris resource *)
 Class nintpGS (Σ : gFunctors) := NintpGS {
+  nintpGS_agreeG :: agreeG (nPropL (;ᵞ)) Σ;
   nintpGS_ninvGS :: ninvGS nInvd Σ;
   nintpGS_na_invG :: na_invG Σ;
   nintpGS_cinvG :: cinvG Σ;
   nintpGS_heapGS :: heapGS_gen HasNoLc Σ;
 }.
-Arguments NintpGS {_} _ _ _ _.
+Arguments NintpGS {_} _ _ _ _ _.
 
 Section nInvd_intp.
   Context `{!nintpGS Σ}.
@@ -50,6 +57,10 @@ Notation "⸨ P ⸩ ( s , i )" := (sunwrap s (Sarg i P%n))
 
 Section iris.
   Context (* Iris resources *) {Σ : gFunctors}.
+
+  Definition nag `{!agreeG (nPropL (;ᵞ)) Σ}
+    (γ : gname) (P : nPropL (;ᵞ)) : iProp Σ :=
+    own γ (to_agree (P : leibnizO _)).
 
   (** [nninv]: [ninv] in the accessor style *)
   Definition nninv_def (s : nsintp_ty Σ)
